\chapter{Exponents}
\begin{exercises}{}{
Simplify without using a calculator:
\begin{multicols}{2}
\begin{enumerate}[label=\textbf{\arabic*}., itemsep=4pt]
 \item $16^0$
 \item $16a^0$
 \item $\dfrac{2^{-2}}{3^2}$
 \item $ \dfrac{5}{2^{-3}}$
 \item $ \left(\dfrac{2}{3}\right)^{-3} $
 \item $ x^2 x^{3t+1} $
 \item $ 3 \times 3^{2a} \times 3^2$
 \item $ \dfrac{a^{3x}}{a^x} $
 \item $ \dfrac{32p^2}{4p^8}$
 \item $ (2t^4)^3$
 \item $ (3^{n+3})^2$
 \item $ \dfrac{3^n 9^{n-3}}{27^{n-1}}$
\end{enumerate}
\end{multicols}
}
\end{exercises}


 \begin{solutions}{}{
\begin{multicols}{2}
\begin{enumerate}[itemsep=5pt, label=\textbf{\arabic*}. ] 


\item $1$
\item $16a^{0}\\
&=16(1)\\
& = 16$
\item \begin{array*}$\dfrac{2^{-2}}{3^2}\\
&=\dfrac{1}{2^2.3^{2}}\\[4pt]
&=\dfrac{1}{4 \times 9}\\[4pt]
&=\dfrac{1}{36}$\end{array*}
\item \begin{array*}$ \dfrac{5}{2^{-3}} \\[4pt]
&=(5)(2^{3})\\
&=(5)(8)\\
&=40$\end{array*}
\item \begin{array*}$ \left(\dfrac{2}{3}\right)^{-3} \\[4pt]
&=\dfrac{2^{−3}}{3^{−3}}\\[4pt]
&=\dfrac{3^3}{2^3}\\[4pt]
&=\dfrac{27}{8}$\end{array*}
\item \begin{array*}$ x^2 x^{3t+1} \\
&=x^{3t+3}$\end{array*}
\item \begin{array*}$3 \times 3^{2a} \times 3^2\\
&=3^{1+2a+2}\\
&=3^{2a+3}$\end{array*}

\item \begin{array*}$\dfrac{a^{3x}}{a^x}\\[4pt]
&=a^{3x}.a^{−x}\\
&=a^{3x−x}\\
&=a^{2x}$\end{array*}
\item \begin{array*}$\dfrac{32p^2}{4p^8}\\[4pt]
&=8p^{2−8}\\
&=8p^{−6}\\[4pt]
&=\dfrac{8}{p^{6}}$\end{array*}
\item \begin{array*}$(2t^4)^3\\
&=2^{3}.t^{4.3}\\
&=8t^{12}$\end{array*}
\item \begin{array*}$(3^{n+3})^2\\
&=3^{2n+6}$\end{array*}
\item \begin{array*}$\dfrac{3^n 9^{n-3}}{27^{n-1}}\\[4pt]
&=\dfrac{3^{n}.(3^{2})^{n−3}}{(3^{3})^{n−1}}\\[4pt]
&=\dfrac{3^{n}.3^{2n−6}}{3^{3n−3}}\\[4pt]
&=3^{n+2n−6−(3n−3)}\\
&=3^{3n−6−3n+3}\\
&=3^{−3}\\[4pt]
&=\dfrac{1}{3^{3}}\\[4pt]
&=\dfrac{1}{27}$\end{array*}

\end{enumerate}
\end{multicols}
}
\end{solutions}


% \section{Rational exponents}
\begin{exercises}{}{
Simplify without using a calculator:
\begin{multicols}{2}
\begin{enumerate}[label=\textbf{\arabic*}., itemsep=5pt]
 \item $ t^{\frac{1}{4}} \times 3t^{\frac{7}{4}} $
 \item $ \dfrac{16x^2}{(4x^2)^{\frac{1}{2}}} $
 \item $ (0,25)^{\frac{1}{2}} $
 \item $ (27)^{-\frac{1}{3}} $
 \item $ (3p^2)^{\frac{1}{2}} \times (3p^4)^{\frac{1}{2}} $
\end{enumerate}
\end{multicols}
}
\end{exercises}


 \begin{solutions}{}{
\begin{multicols}{2}
\begin{enumerate}[itemsep=5pt, label=\textbf{\arabic*}. ] 


\item \begin{array*}$t^{\frac{1}{4}} \times 3t^{\frac{7}{4}}\\
&=3t^{(\frac{1}{4}+\frac{7}{4})}\\
&=3t^{\frac{8}{4}}\\
&=3t^{2}$\end{array*}
\item \begin{array*}$\dfrac{16x^2}{(4x^2)^{\frac{1}{2}}}\\[4pt]
&=\dfrac{16x^{2}}{4^{\frac{1}{2}} x^{2{\frac{1}{2}}}}\\[4pt]
&=\dfrac{4^{2}x^{2}}{4^{\frac{1}{2}}x}\\[4pt]
&=4^{2−\frac{1}{2}}.x^{2−1}\\
&=4^{\frac{3}{2}}.x\\
&=(2^{2})^{\frac{3}{2}}x\\
&=2^{3}x\\
&=8x$\end{array*}
\item \begin{array*}$(0,25)^{\frac{1}{2}}\\
&=\left(\frac{1}{4}\right)^{\frac{1}{2}}\\
&=\left(\frac{1}{2^2}\right)^{\frac{1}{2}}\\
&=\left(2^{−2}\right)^{\frac{1}{2}}\\
&=2−1\\
&=\frac{1}{2}$\end{array*}
\item \begin{array*}$(27)^{-\frac{1}{3}}\\
&=(3^{3})^{−\frac{1}{3}}\\
&=3^{−1}\\
&=\frac{1}{3}$\end{array*}
\item \begin{array*}$(3p^2)^{\frac{1}{2}} \times (3p^4)^{\frac{1}{2}} \\
&=3^{\frac{1}{2}}p \times 3^{\frac{1}{2}}p^{2}\\
&=3^{\frac{1}{2}+\frac{1}{2}} \times p^{1+2}\\
&=3p^{3}$\end{array*}

\end{enumerate}
\end{multicols}
}
\end{solutions}


% \section{Exponential equations}
\begin{exercises}{}{
\begin{enumerate}[label=\textbf{\arabic*}., itemsep=5pt]
\item Solve for the variable:
\begin{enumerate}[label=\textbf{(\alph*)}, itemsep=4pt]
\begin{multicols}{2}
\item $ 2^{x+5} = 32 $
\item $ 5^{2x+2} = \dfrac{1}{125} $
\item $ 64^{y+1} = 16^{2y+5} $
\item $ 3^{9x-2} = 27 $
\item $ 81^{k+2} = 27^{k+4} $
\item $ 25^{(1-2x)}-5^4 = 0 $
\item $ 27^x \times 9^{x-2} = 1 $
\item $ 2^t + 2^{t+2} = 40 $
\item $ 2 \times 5^{2-x} = 5+ 5^x $
\item $ 9^m + 3^{3-2m} = 28 $
\item $ y - 2y^{\frac{1}{2}} + 1 = 0 $
\item $4^{x+3} = 0,5$
\item $2^a = 0,125$
\item $10^x = 0,001$
\item $2^{x^2-2x-3} = 1$
\end{multicols}
\end{enumerate}
 \item The growth of algae can be modelled by the function $f(t) = 2^t$. Find the value of $t$ such that $f(t)=128$.   
\end{enumerate}

}
\end{exercises}


 \begin{solutions}{}{
\begin{enumerate}[itemsep=5pt, label=\textbf{\arabic*}. ] 


\item 
\begin{multicols}{2}
\begin{enumerate}[label=\textbf{(\alph*)}, itemsep=5pt]
\item \begin{array*}$2^{x+5}&=&32\\
2^{x+5}&=&2^{5}\\
x+5&=&5\\
x&=&0$\end{array*}
\item \begin{array*}$5^{2x+2}=\dfrac{1}{125}\\[4pt]
5^{2x+2}=\dfrac{1}{5^3}\\[4pt]
5^{2x+2}=5^{−3}\\
2x+2=−3\\
2x=−5\\
x=−\frac{5}{2} $\end{array*}
\item \begin{array*}$64^{y+1}=16^{2y+5}\\
2^{6(y+1)}=2^{4(2y+5)}\\
2^{6y+6}=2^{8y+20}\\
6y+6=8y+20\\
6y−8y=20−6\\
−2y=14\\
y=−7$\end{array*}
\item \begin{array*}$3^{9x−2}=27\\
3^{9x−2}=3^{3}\\
9x−2=3\\
9x=5\\
x=\frac{5}{9}$\end{array*}
\item \begin{array*}$81^{k+2}=27^{(k+4)}\\
3^{4(k+2)}=3^{3(k+4)}\\
3^{4k+8}=3^{3k+12}\\
4k+8=3k+12\\
4k−3k=12−8\\
k=4$\end{array*}
\item \begin{array*} $25^{(1−2x)}−5^{4}=0\\
5^{2(1−2x)}=5^{4}\\
2(1−2x)=4\\
1−2x=2\\
−2x=1\\
x=−\frac{1}{2}$\end{array*}
\item \begin{array*}$27^{x} \times 9^{x−2}=1\\
3^{3x} \times 3^{2(x−2)}=1\\
3^{3x+2(x−2)}=3^{0}\\
3x+2x−4=0\\
5x−4=0\\
5x=4\\
x=\dfrac{4}{5} $\end{array*}
\item \begin{array*}$2^{t}+2^{t+2}=40\\
2^{t}+2^{t}.2^{2}=40\\
2^{t}(1+2^{2})=40\\
2^{t}(1+4)=40\\
2^{t}=\dfrac{40}{(1+4)}\\[4pt]
2^{t}=\dfrac{40}{5}\\[4pt]
2^{t}=8\\
2^{t}=2^{3}\\
t=3$\end{array*}
\item \begin{array*}$2.5^{2−x}=5+5^{x}\\
2.5^{2}.5^{−x}=5+5^{x}\\[4pt]
\dfrac{2.5^2}{5^x}−5−5^{x}=0\\[4pt]
\left(\frac{50}{5^{x}}\right) \times 5^{x} − 5 \times (5^{x})−5^{x} \times (5^{x})=0\\[4pt]
50−5.5^{x}−(5^{x})^{2}=0\\
(5^{x})^{2}+5.5^{x}−50=0\\
(5^{x}−5)(5^{x}+10)=0\\
5^{x}−5=0~\mbox{ or }~5^{x}+10=0\\
5^{x}=5~\mbox{ or } ~5^{x}=−10\\
\mbox{if }~5^{x}=−10:~ \mbox{ no solution}\\
\mbox{if }~5^{x}=5:\\
5^{x}=5^{1}\\
x=1$\end{array*}
\item \begin{array*}$9^{m}+3^{3−2m}=28\\
3^{2m}+3^{3}.3^{−2m}=28\\[4pt]
3^{2m}+\dfrac{27}{3^{2m}}−28=0\\[4pt]
(3^{2m})^{2}−28(3^{2m})+27=0\\
(3^{2m}−27)(3^{2m}−1)=0\\
3^{2m}−27=0~\mbox{ or }~3^{2m}−1=0\\
3^{2m}=27~\mbox{ or }~3^{2m}=1\\
\mbox{if }~3^{2m}=27\\
3^{2m}=3^{3}\\
2m=3\\
m=\frac{3}{2}\\
\mbox{if }~3^{2m}=1\\
3^{2m}=3^{0}\\
2m=0\\
m=0$\end{array*}
\item \begin{array*}$ y−2y^{\frac{1}{2}}+1=0\\
(y^{\frac{1}{2}}−1)(y^{\frac{1}{2}}−1)=0\\
y^{\frac{1}{2}}−1=0\\
y^{\frac{1}{2}}=1\\
y^{\frac{1}{2}}=1^{\frac{1}{2}}\\
y=1 $\end{array*}
\item $4^{x+3} = 0,5\\
2^{2x+6} = 2^{-1}\\
2x+6=-1\\
2x=-7\\
x=-3\frac{1}{2}$
\item $2^a = 0,125\\
2^a = \frac{125}{1000}\\
2^a = \frac{1}{8}\\
2^a = \frac{1}{2^3}\\
2^a=2^{-3}\\
a=-3$
\item $10^x = 0,001\\
10^{x} = \frac{1}{1000}\\
=\frac{1}{10^3}\\
=10^{-3}\\
x=-3$
\item $2^{x^2-2x-3} = 1\\
2^{x^2-2x-3}=2^0\\
x^2-2x-3=0\\
(x-3)(x+1)=0\\
x=3$ or $x=-1$
\end{enumerate}
\end{multicols}
\item $2^{t}=128\\
2^{t}=2^{7}\\
t=7$

\end{enumerate}}
\end{solutions}


\begin{eocexercises}{}
\begin{enumerate}[label=\textbf{\arabic*}., itemsep=5pt]
\item Simplify:
\begin{multicols}{2}
\begin{enumerate}[label=\textbf{(\alph*)}, itemsep=6pt]
\item $ t^3 \times 2t^0 $
\item $ 5^{2x+y} 5^{3(x+z)} $
\item $ (b^{k+1})^k $
\item $ \dfrac{6^{5p}}{9^p} $
\item $ m^{-2t} \times (3m^t)^3 $
\item $\dfrac{3{x}^{-3}}{{(3x)}^{2}}$
\item $\dfrac{{5}^{b-3}}{{5}^{b+1}}$
\item $\dfrac{{2}^{a-2} {3}^{a+3}}{{6}^{a}}$
\item $\dfrac{{3}^{n} {9}^{n-3}}{{27}^{n-1}}$
\item ${\left(\dfrac{2{x}^{2a}}{{y}^{-b}}\right)}^{3}$
\item $\dfrac{{2}^{3x-1} {8}^{x+1}}{{4}^{2x-2}}$
\item $\dfrac{{6}^{2x} {11}^{2x}}{{22}^{2x-1} {3}^{2x}}$
\item $\dfrac{{(-3)}^{-3} {(-3)}^{2}}{{(-3)}^{-4}}$
\item ${({3}^{-1}+{2}^{-1})}^{-1}$
\item $\dfrac{{9}^{n-1} {27}^{3-2n}}{{81}^{2-n}}$
\item $\dfrac{{2}^{3n+2} {8}^{n-3}}{{4}^{3n-2}}$
\item $\dfrac{3^{t+3} + 3^t}{2 \times 3^t} $
\item $\dfrac{2^{3p} +1}{2^p + 1} $
\end{enumerate}
\end{multicols}
\item Solve:
\begin{multicols}{2}
\begin{enumerate}[label=\textbf{(\alph*)}, itemsep=6pt]
\setcounter{enumi}{18}
\item $ 3^x = \dfrac{1}{27} $
\item $ 5^{t-1} = 1 $
\item $ 2 \times 7^{3x} = 98 $
\item $ 2^{m+1} = (0,5)^{m-2}$
\item $ 3^{y+1} = 5^{y+1} $
\item $ z^{\frac{3}{2}} = 64 $
\item $ 16x^{\frac{1}{2}} - 4 = 0 $
\item $ m^0 + m^{-1} = 0 $
\item $ t^{\frac{1}{2}} - 3t^{\frac{1}{4}} + 2 = 0 $
\item $ 3^p + 3^p + 3^p = 27 $
\item $ k^{-1} - 7k^{-\frac{1}{2}} -18 = 0 $
\item $ x^{\frac{1}{2}}+3x^{\frac{1}{4}}-18 = 0 $
\end{enumerate}
\end{multicols}

\end{eocexercises}


 \begin{eocsolutions}{}{
\begin{enumerate}[itemsep=7pt, label=\textbf{\arabic*}. ] 


\item 
\begin{multicols}{2}
\begin{enumerate}[label=\textbf{(\alph*)}, itemsep=10pt]

%a
\item $ t^3 \times 2t^{0}\\
=t^{3} \times 2(1) \\
=2t^3 $
%b
\item $5^{2x+y}\times5^{3(x+z)}\\
=5^{2x+y+3x+3z}\\
=5^{5x+y+3z}$
%c
\item $\left(b^{k+1}\right)^{k}=b^{k^{2}+k}$
%d
\item $ \dfrac{6^{5p}}{9^p}\\[4pt]
=\dfrac{2^{5p}\times3^{5p}}{3^{2p}}\\[4pt]
=2^{5p}\times3^{5p−2p}\\
=2^{5p}\times3^{3p}\\
=\left(2^{5}\times3^{3}\right)^{p}\\
=\left(32 \times 27\right)^{p}\\
=864^{p}$
%e
\item $m^{−2t} \times \left(3m^{t}\right)^{3}\\
=m^{−2t} \times 3^{3}m^{3t}\\
=m^{−2t+3t}\times27\\
=27m^{t}$
%f
\item $\dfrac{3x^{−3}}{(3x)^{2}}\\[4pt]
=3^{1−2}\times x^{−3−2}\\
=3^{−1}\times x^{−5}\\
=\dfrac{1}{3x^{5}}$
%g
\item $\dfrac{{5}^{b-3}}{{5}^{b+1}}\\[4pt]
=5^{b−3−b−1}\\
=5^{−4}\\
=\dfrac{1}{5^{4}}\\[4pt]
=\dfrac{1}{625}$
%h
\item $\dfrac{{2}^{a-2} {3}^{a+3}}{{6}^{a}}\\[4pt]
=\dfrac{2^{a−2}\times3^{a+3}}{(2\times3)^{a}}\\[4pt]
=\dfrac{2^{a−2}\times3^{a+3}}{2^{a}\times3^{a}}\\[4pt]
=2^{a−2−a}\times3^{a+3−a}\\
=2^{−2}\times3^{3}\\
=\dfrac{3^3}{2^2}\\[4pt]
=\dfrac{27}{4}$
%i
\item $\dfrac{{3}^{n} {9}^{n-3}}{{27}^{n-1}}\\[4pt]
=\dfrac{3^{n}\times\left(3^{2}\right)^{n−3}}{\left(3^{3}\right)^{n−1}}\\[4pt]
=\dfrac{3^{n}\times3^{2n−6}}{3^{3n−3}}\\[4pt]
=3^{n+2n−6−(3n−3)}\\
=3^{3n−6−3n+3}\\
=3^{−3}\\
=\dfrac{1}{3^{3}}\\[4pt]
=\dfrac{1}{27}$
%j
\item ${\left(\dfrac{2{x}^{2a}}{{y}^{-b}}\right)}^{3}\\[4pt]
=\dfrac{2^{3}\left(x^{2a}\right)^{3}}{\left(y^{−b}\right)^{3}}\\[4pt]
=\dfrac{2^{3}x^{6a}}{y^{−3b}}\\[4pt]
=2^{3}x^{6a}y^{3b}\\
=8x^{6a}y^{3b}$
%k
\item $\dfrac{{2}^{3x-1} {8}^{x+1}}{{4}^{2x-2}}\\[4pt]
=\dfrac{2^{3x−1}\times2^{3(x+1)}}{2^{2(2x−2)}}\\[4pt]
=2^{3x−1+3x+3−4x+4}\\
=2^{2x+6}\\
=4^{x+3}$
%l
\item $\dfrac{{6}^{2x} {11}^{2x}}{{22}^{2x-1} {3}^{2x}}\\[4pt]
=\dfrac{(3\times2)^{2x}\times11^{2x}}{(2\times11)^{2x−1}\times3^{2x}}\\[4pt]
=\dfrac{3^{2x}\times2^{2x}\times11^{2x}}{2^{2x−1}\times11^{2x−1}\times3^{2x}}\\[4pt]
=3^{2x−2x}\times2^{2x−2x+1}\times11^{2x−2x+1}\\
=3^{0}\times2^{1}\times11^{1}\\
=1\times2\times11\\
=22$
%m
\item $\dfrac{{(-3)}^{-3} {(-3)}^{2}}{{(-3)}^{-4}}\\[4pt]
=(−3)^{−3+2+4}\\
=(−3)^{3}\\
=−27$
%n
\item ${({3}^{-1}+{2}^{-1})}^{-1}\\
=\left(\dfrac{1}{3}+\dfrac{1}{2}\right)^{−1}\\[4pt]
=\left(\dfrac{2}{6}+\dfrac{3}{6}\right)^{−1}\\[4pt]
=\left(\dfrac{5}{6}\right)^{−1}\\[4pt]
=\left(\dfrac{5^{−1}}{6^{−1}}\right)\\[4pt]
=\dfrac{6}{5}$
%o
\item $\dfrac{{9}^{n-1} {27}^{3-2n}}{{81}^{2-n}}\\[4pt]
=\dfrac{3^{2(n−1)}\times3^{3(3−2n)}}{3^{4(2−n)}}\\[4pt]
=3^{2(n−1)+3(3−2n)−4(2−n)}\\
=3^{2n−2+9−6n−8+4n}\\
=3^{−1}\\[4pt]
=\dfrac{1}{3}$
%p
\item $\dfrac{{2}^{3n+2} {8}^{n-3}}{{4}^{3n-2}}\\[4pt]
=\dfrac{2^{3n+2}\times2^{3(n−3)}}{2^{2(3n−2)}}\\[4pt]
=2^{3n+2+3(n−3)−2(3n−2)}\\
=2^{3n+2+3n−9−6n+4}\\
=2^{−3}\\
=\dfrac{1}{2^{3}}\\[4pt]
=\dfrac{1}{8}$
%q
\item $\dfrac{3^{t+3} + 3^t}{2 \times 3^t} \\[4pt]
=\dfrac{3^{t}\times3^{3}+3^{t}}{2\times3^{t}}\\[4pt]
=\dfrac{3^{t}(3^{3}+1)}{2\times3^{t}}\\[4pt]
=\dfrac{3^{3}+1}{2}\\[4pt]
=\dfrac{28}{2}\\[4pt]
=14$
%r
\item $\dfrac{2^{3p} +1}{2^p + 1} \\[4pt]
=\dfrac{(2^{p}+1)(2^{2p}−2^{p}+1)}{(2^{p}+1)}\\[4pt]
=2^{2p}−2^{p}+1$
\end{enumerate}
\end{multicols}
\item 
\begin{multicols}{2}
\begin{enumerate}[label=\textbf{(\alph*)}, itemsep=7pt]
% \setcounter{enumi}{18}
%a
\item $ 3^x = \dfrac{1}{27} \\[4pt]
3^{x}=\dfrac{1}{3^{3}}\\[4pt]
3^{x}=3^{−3}\\
x=-3$
%b
\item $5^{t−1}=1\\
5^{t−1}=5^{0}\\
t−1=0\\
t=1$
%c
\item $ 2 \times 7^{3x} = 98 \\
7^{3x}=49\\
7^{3x}=7^{2}\\
3x=2\\
x=\frac{2}{3}$
%d
\item $ 2^{m+1} = (0,5)^{m-2}\\
2^{m+1}=\left(\frac{1}{2}\right)^{m−2}\\
2^{m+1}=\left(2^{−1}\right)^{m−2}\\
2^{m+1}=\left(2\right)^{2−m}\\
m+1=2−m\\
2m=1\\
m=\frac{1}{2}$
%e
\item $ 3^{y+1} = 5^{y+1} \\
y+1=0\\
y=−1$
%f
\item $ z^{\frac{3}{2}} = 64 \\
z^{\frac{3}{2}}=4^{3}\\[3pt]	
\left(z^{\frac{3}{2}}\right)^{\frac{2}{3}}=(4^{3})^{\frac{2}{3}}\\
z=4^{2}\\
z=16$
%g
\item $ 16x^{\frac{1}{2}} - 4 = 0 \\
16x^{\frac{1}{2}}=4\\
x^{\frac{1}{2}}=\frac{4}{16}\\
x^{\frac{1}{2}}=\frac{1}{4}\\
\left(x^{\frac{1}{2}}\right)^{2}=\left(\frac{1}{4}\right)^2\\
x=\frac{1}{16}$
%h
\item $ m^0 + m^{-1} = 0 \\
1+m^{−1}=0\\
m^{−1}=−1\\
\left(m^{−1}\right)^{−1}=(−1)^{−1}\\
m=−1$
%i
\item $ t^{\frac{1}{2}} - 3t^{\frac{1}{4}} + 2 = 0 \\
(t^{\frac{1}{4}}−1)(t^{\frac{1}{4}}−2)\\
t^{\frac{1}{4}}−1=0~\mbox{ or }~t^{\frac{1}{4}}−2=0\\
\mbox{if }~t^{\frac{1}{4}}−1=0:\\
t^{\frac{1}{4}}=1\\
\left(t^{\frac{1}{4}}\right)^{4}=1^{4}\\
t=1\\
\mbox{if }~t^{\frac{1}{4}}−2=0:\\
t^{\frac{1}{4}}=2\\
\left(t^{\frac{1}{4}}\right)^{4}=2^{4}\\
t=16$
%j
\item $ 3^p + 3^p + 3^p = 27 \\
3\times3^{p}=27\\
3^{p+1}=3^{3}\\
p+1=3\\
p=2$
%k
\item $ k^{-1} - 7k^{-\frac{1}{2}} -18 = 0 \\
(k^{-\frac{1}{2}}−9)(k^{-\frac{1}{2}}+2)=0\\
k^{-\frac{1}{2}}−9=0~\mbox{ or }~k^{-\frac{1}{2}}+2=0\\
k^{-\frac{1}{2}}=9 ~\mbox{ or }~k^{-\frac{1}{2}}=−2\\
\mbox{if }~k^{-\frac{1}{2}}=9:\\
(k^{-\frac{1}{2}})^{−2}=9^{−2}\\
k=\frac{1}{81}\\
\mbox{if }~k^{-\frac{1}{2}}=−2:\\
(k^{-\frac{1}{2}})^{−2}=(−2)^{−2}\\
k=\frac{1}{4}$
%l
\item $ x^{\frac{1}{2}}+3x^{\frac{1}{4}}-18 = 0 \\
(x^{\frac{1}{4}}+6)(x^{\frac{1}{4}}−3)=0\\
x^{\frac{1}{4}}+6=0~\mbox{ or }~x^{\frac{1}{4}}−3=0\\
x^{\frac{1}{4}}=−6~\mbox{ or }~x^{\frac{1}{4}}=3\\
\mbox{if }~x^{\frac{1}{4}}=−6:\\
\left(x^{\frac{1}{4}}\right)^{4}=(−6)^{4}\\
x=1296\\
\mbox{if }~x^{\frac{1}{4}}=3:\\
(x^{\frac{1}{4}})^{4}=(3)^{4}\\
x=81$
\end{enumerate}
\end{multicols}

\end{enumerate}}
\end{eocsolutions}


